finish A3

a3/dafny/SlowMax.dfy
@@ -1,17 +1,19 @@
-function max(x:nat, y:nat) : nat
-{
+function max(x:nat, y:nat) : nat {
   if (x < y) then y else x
 }
 
 method slow_max(a: nat, b: nat) returns (z: nat)
-  ensures z == max(a, b)
-{
+  ensures z == max(a, b) {
   z := 0;
   var x := a;
   var y := b;
   while (z < x && z < y)
-    invariant true 
-    decreases 0
+    invariant (a-x) == (b-y)
+    invariant z == (a-x) || z == (b -y)
+    invariant 0<= x <= a
+    invariant 0<= y <= b
+    decreases x
+    decreases y
   {
     z := z + 1;
     x := x - 1;
