a3/dafny/CalcTerm.dfy
@@ -17,18 +17,19 @@ method CalcTerm(m: int, n: nat) returns (res: int)
   res := 0;
 
   while (m1!=0)
-    invariant true
-    decreases 0
+    invariant res == (abs(m)-m1)*5
+    decreases m1
   {
     res := res+5;
     m1 := m1-1;
   }
 
   if (m<0) { res := -res; }
+  var ori := res;
 
   while (n1!=0)
-    invariant true
-    decreases 0
+    invariant res == ori - 3 * (n - n1);
+    decreases n1;
   {
     res := res-3;
     n1 := n1-1;
