a3/dafny/pancakesort/PancakeSort.dfy
@@ -3,11 +3,17 @@ include "findmax.dfy"
 
 
 method pancakeSort (a : array<int>)
+  requires a != null && a.Length > 0;
   modifies a;
   ensures forall i, j :: 0 <= i <= j < a.Length ==> a[i] <= a[j];
 {
   var curr_size := a.Length;
   while (curr_size > 1)
+    decreases curr_size;
+    invariant 1 <= curr_size <= a.Length;
+    invariant multiset(old(a[..])) == multiset(a[..]);
+    invariant forall i, j :: 0 <= i < curr_size <= j < a.Length ==> a[i] <= a[j];
+    invariant forall i, j :: curr_size <= i <= j < a.Length ==> a[i] <= a[j];
   {
     var mi := findMax (a, curr_size);
     if (mi != curr_size - 1)
