a3/dafny/pancakesort/findmax.dfy
@@ -1,11 +1,19 @@
 // returns an index of the largest element of array 'a' in the range [0..n)
 method findMax (a : array<int>, n : int) returns (r:int)
+  requires a != null && a.Length > 0;
+  requires 0 < n <= a.Length;
+  ensures 0 <= r < n;
+  ensures forall j :: 0 <= j < n ==> a[j] <= a[r]
 {
   var mi;
   var i;
   mi := 0;
   i := 0;
   while (i < n)
+    invariant 0 <= i <= n;
+    invariant 0 <= mi < n;
+    decreases n-i;
+    invariant forall k :: 0 <= k < i ==> a[k] <= a[mi]
   {
     if (a[i] > a[mi])
     { mi := i; }
