a3/dafny/pancakesort/flip.dfy
@@ -1,11 +1,25 @@
 // flips (i.e., reverses) array elements in the range [0..num]
 method flip (a: array<int>, num: int)
+  requires a != null && a.Length > 0;
+  requires 0 <= num < a.Length;
+  modifies a;
+  ensures multiset(old(a[..])) == multiset(a[..]);
+  ensures forall p :: 0 <= p <= num  ==> a[p] == old(a[num-p]);
+  ensures forall p :: num < p < a.Length ==> a[p] == old(a[p]);
 {
   var tmp:int;
-
   var i := 0;
   var j := num;
   while (i < j)
+    decreases num - i;
+    invariant i + j ==num;
+    invariant 0 <= i <= num/2 + 1;
+    invariant num/2-1 <= j <=num;
+    invariant multiset(old(a[..])) == multiset(a[..]);
+    invariant forall p :: 0<= p <i ==> a[p] == old(a[num-p]);
+    invariant forall p :: num < p < a.Length ==> a[p] == old(a[p]);
+    invariant forall p :: 0<= p <i ==> a[num-p] == old(a[p]);
+    invariant forall p :: i<= p <= j ==> a[p] == old(a[p]);
   {
     tmp := a[i];
     a[i] := a[j];
